src/Manifest_JSON.v
@@ -47,29 +47,23 @@ Global Instance Jsonifiable_Manifest : Jsonifiable Manifest :=
   }.
 
 Definition AM_Lib_to_JSON (am : AM_Library) : JSON :=
-  let '(Build_AM_Library clone_uuid lib_asps lib_appr_asps lib_plcs lib_pubkeys) := am
+  let '(Build_AM_Library clone_uuid lib_plcs lib_pubkeys) := am
   in
     JSON_Object [
       (AM_CLONE_UUID, (InJSON_String (to_string clone_uuid)));
-      (AM_LIB_ASPS, (InJSON_Object (to_JSON lib_asps)));
-      (AM_LIB_APPR_ASPS, (InJSON_Array (map_pair_to_InnerJSON_string lib_appr_asps)));
       (AM_LIB_PLCS, (InJSON_Object (to_JSON lib_plcs)));
       (AM_LIB_PUBKEYS, (InJSON_Object (to_JSON lib_pubkeys)))
     ].
 
 Definition JSON_to_AM_Lib (js : JSON) : ResultT AM_Library string :=
   temp_CLONE_UUID <- JSON_get_string AM_CLONE_UUID js;;
-  temp_LIB_ASPS <- JSON_get_Object AM_LIB_ASPS js;;
-  temp_LIB_APPR_ASPS <- JSON_get_Array AM_LIB_APPR_ASPS js;;
   temp_LIB_PLCS <- JSON_get_Object AM_LIB_PLCS js;;
   temp_LIB_PUBKEYS <- JSON_get_Object AM_LIB_PUBKEYS js;;
 
   CLONE_UUID <- from_string temp_CLONE_UUID;;
-  LIB_ASPS <- from_JSON temp_LIB_ASPS;;
-  LIB_APPR_ASPS <- InnerJson_string_to_map_pair temp_LIB_APPR_ASPS;;
   LIB_PLCS <- from_JSON temp_LIB_PLCS;;
   LIB_PUBKEYS <- from_JSON temp_LIB_PUBKEYS;;
-  resultC (Build_AM_Library CLONE_UUID LIB_ASPS LIB_APPR_ASPS LIB_PLCS LIB_PUBKEYS).
+  resultC (Build_AM_Library CLONE_UUID LIB_PLCS LIB_PUBKEYS).
 
 Global Instance Jsonifiable_AM_Library : Jsonifiable AM_Library :=
   { to_JSON := AM_Lib_to_JSON;
